CCsub_Subcapt.v
@@ -1,4 +1,5 @@
 Require Import Coq.Program.Equality.
+Require Import LibTactics.
 Require Export CCsub_Hints.
 Require Export CCsub_Lemmas.
 
@@ -87,23 +88,35 @@ Proof with eauto.
   eapply subcapt_reflexivity...
 Qed.
 
+(* TODO: move to lemmas.v *)
+Lemma pure_type_empty_cv : forall T,
+  pure_type T ->
+  typ_cv T = {}.
+Proof.
+  intros * Hpure.
+  inversion Hpure; simpl; reflexivity.
+Qed.
+
 (* Subtyping implies subcapturing *)
 Lemma sub_implies_subcapt : forall Γ S T,
   Γ ⊢ S <: T ->
   Γ ⊢ₛ (typ_cv S) <: (typ_cv T).
-Local Ltac hint ::=
-  eauto using subcapt_reflexivity.
-Proof with hint.
+Proof with eauto using subcapt_reflexivity.
   intros * Hsub.
   assert (Γ ⊢ₛ (typ_cv S) wf); [apply cv_wf|]...
   assert (Γ ⊢ₛ (typ_cv T) wf); [apply cv_wf|]...
   induction Hsub; simpl in *...
-  - Case "sub_trans_tvar".
-    apply subcapt_empty...
-  - Case "sub_top".
-    (* REVIEW: not true, this lemma only works for non pure types *)
-    admit.
-Admitted.
+  - rename select (binds X _ _) into Binds.
+    assert (WfEnv : Γ ⊢ wf) by (applys sub_regular Hsub).
+    assert (PureU : pure_type U) by (applys wf_typ_env_bind_sub WfEnv Binds).
+    replace (typ_cv T) with {}...
+    symmetry.
+    apply pure_type_empty_cv.
+    applys sub_pure_type Hsub.
+    apply PureU.
+  - rename select (pure_type T) into PureT.
+    rewrite (pure_type_empty_cv _ PureT)...
+Qed.
 
 (* Substituting the same capture set preserves subcapturing *)
 Lemma subcapt_through_subst_cset : forall x U C Δ Γ C1 C2 ,
@@ -125,7 +138,7 @@ Proof with eauto using wf_env_subst_cb, wf_cset_subst_cb with fsetdec.
     destruct_set_mem x xs.
     + assert ((Δ ++ [(x, bind_typ U)] ++ Γ) ⊢ U wf) as HA. {
         note (wf_env ([(x, bind_typ U)] ++ Γ)) by eauto...
-        rewrite_env (∅ ++ (Δ ++ [(x, bind_typ U)]) ++ Γ).
+        rewrite_env (∅ ++ (Δ ++ [(x, bind_typ (C1 # R))]) ++ Γ).
         apply wf_typ_weakening; simpl_env...
       }
       forwards: cv_wf HA.
@@ -146,7 +159,7 @@ Proof with eauto using wf_env_subst_cb, wf_cset_subst_cb with fsetdec.
       2: exfalso; fsetdec.
       assert ((Δ ++ [(x, bind_typ U)] ++ Γ) ⊢ₛ C wf) as HA. {
         note (([(x, bind_typ U)] ++ Γ) ⊢ wf) by eauto...
-        rewrite_env (∅ ++ (Δ ++ [(x, bind_typ U)]) ++ Γ).
+        rewrite_env (∅ ++ (Δ ++ [(x, bind_typ (C0 # R))]) ++ Γ).
         apply wf_cset_weakening; simpl_env...
       }
       inversion HA; subst.
@@ -163,7 +176,7 @@ Proof with eauto using wf_env_subst_cb, wf_cset_subst_cb with fsetdec.
       }
       assert ((Δ ++ [(x, bind_typ U)] ++ Γ) ⊢ₛ C wf) as HA. {
         note (([(x, bind_typ U)] ++ Γ) ⊢ wf) by eauto...
-        rewrite_env (∅ ++ (Δ ++ [(x, bind_typ U)]) ++ Γ).
+        rewrite_env (∅ ++ (Δ ++ [(x, bind_typ (C0 # R))]) ++ Γ).
         apply wf_cset_weakening; simpl_env...
       }
       note (Γ ⊢ₛ C wf).
@@ -188,126 +201,58 @@ Proof with eauto using wf_env_subst_cb, wf_cset_subst_cb with fsetdec.
     + assert (x0 = x) by fsetdec; subst.
       assert (binds x (bind_typ U) (Δ ++ [(x, bind_typ U)] ++ Γ)) as HA by auto.
       forwards EQ: binds_typ_unique H HA; subst; clear HA.
-      assert (Γ ⊢ U wf) by eauto.
+      assert (Γ ⊢ (C1 # R) wf).
+      { apply wf_env_tail in WfE.
+        inversion WfE...
+      }
       assert (x ∉ dom Γ) as HA. {
-        assert (ok (Δ ++ [(x, bind_typ U)] ++ Γ)) as HA by auto.
+        assert (ok (Δ ++ [(x, bind_typ (C1 # R))] ++ Γ)) as HA by auto.
         apply ok_tail in HA.
         inversion HA...
       }
-      forwards: notin_fv_wf_typ H0 HA.
+      forwards NotIn: notin_fv_wf_typ H0 HA.
       replace (C `u` cset_set ({x}A `\`A x) {}N false)
-              with C by (destruct U; csetdec).
-      apply (subcapt_transitivity (typ_cv U))... {
+              with C by csetdec.
+      apply (subcapt_transitivity C1)... {
         rewrite_env (∅ ++ (map (subst_cb x C) Δ ++ Γ)).
         apply subcapt_weakening; simpl_env...
       }
-      replace (typ_cv U) with (subst_cset x C (typ_cv U)).
-      2: {
-        symmetry.
-        apply subst_cset_fresh.
-        destruct U; simpl in *; csetdec.
-        destruct v.
-        - simpl in H2.
-          apply (H1 H2).
-        - simpl in H2.
-          fsetdec. 
-      }
+      simpl in NotIn.
+      replace C1 with (subst_cset x C C1)
+        by (symmetry; apply subst_cset_fresh; fsetdec).
       eapply IHHsc...
     + assert (x0 <> x) by fsetdec.
       binds_cases H.
       * specialize (IHHsc x U Δ Γ ltac:(trivial) ltac:(trivial)).
         forwards: wf_typ_from_binds_typ H...
-        eapply subcapt_var with (T := T)...
-        replace (typ_cv T) with (subst_cset x C (typ_cv T)).
-        2: {
-          symmetry; apply subst_cset_fresh.
-          assert (x ∉ dom Γ) as HA. {
-            assert (ok (Δ ++ [(x, bind_typ U)] ++ Γ)) as HA by auto.
-            apply ok_tail in HA.
-            inversion HA...
-          }
-          forwards: notin_fv_wf_typ H1 HA.
-          destruct T; simpl in *; try fsetdec.
-          destruct v; simpl...
-        }
-        apply IHHsc...
-      * assert (binds x0 (bind_typ (subst_ct x C T)) (map (subst_cb x C) Δ ++ Γ)) as HBnd by auto.
         eapply subcapt_var...
-        replace (typ_cv (subst_ct x C T))
-          with (subst_cset x C (typ_cv T)).
-        2: {
-          destruct T; simpl; unfold subst_cset...
-          destruct v; simpl.
-          2-6: destruct_set_mem x {}A; [ clear - xIn0; exfalso; fsetdec | reflexivity ].
-          assert (x <> a). {
-            forwards WfA: wf_typ_from_binds_typ x0 a...
-            assert (binds x _ (Δ ++ [(x, bind_typ U)] ++ Γ)) by auto.
-            inversion WfA; subst.
-            forwards: binds_unique a...
-          }
-          unfold subst_cset.
-          destruct_set_mem x {a}A; [exfalso;fsetdec|].
-          easy.
-        }
-        eapply IHHsc...
-  - Case "subcapt_tvar".
-    unfold subst_cset at 1.
-    destruct_set_mem x (singleton x0).
-    + assert (x0 = x) by fsetdec; subst.
-      assert (binds x (bind_typ U) (Δ ++ [(x, bind_typ U)] ++ Γ)) as HA by auto.
-      forwards EQ: binds_unique H HA.
-      exfalso;congruence.
-    + assert (x0 <> x) by fsetdec.
-      binds_cases H.
-      * specialize (IHHsc x U Δ Γ ltac:(trivial) ltac:(trivial)).
-        forwards: wf_typ_from_binds_sub H...
-        eapply subcapt_tvar with (T := T)...
-        replace (typ_cv T) with (subst_cset x C (typ_cv T)).
-        2: {
-          symmetry; apply subst_cset_fresh.
-          assert (x ∉ dom Γ) as HA. {
+        assert (x ∉ dom Γ) as HA. {
             assert (ok (Δ ++ [(x, bind_typ U)] ++ Γ)) as HA by auto.
             apply ok_tail in HA.
             inversion HA...
           }
-          forwards: notin_fv_wf_typ H1 HA.
-          destruct T; simpl in *; try fsetdec.
-          destruct v; simpl...
-        }
+        forwards NotIn: notin_fv_wf_typ H1 HA.
+        simpl in NotIn.
+        replace C1 with (subst_cset x C C1)
+          by (symmetry; apply subst_cset_fresh; fsetdec).
         apply IHHsc...
-      * assert (binds x0 (bind_sub (subst_ct x C T)) (map (subst_cb x C) Δ ++ Γ)) as HBnd by auto.
-        eapply subcapt_tvar...
-        replace (typ_cv (subst_ct x C T)) with (subst_cset x C (typ_cv T)).
-        2: {
-          destruct T; simpl; unfold subst_cset...
-          destruct v; simpl.
-          2-6: destruct_set_mem x {}A; [ clear - xIn0; exfalso; fsetdec | reflexivity ].
-          assert (x <> a). {
-            forwards WfA: wf_typ_from_binds_sub x0 a...
-            assert (binds x _ (Δ ++ [(x, bind_typ U)] ++ Γ)) by auto.
-            inversion WfA; subst.
-            forwards: binds_unique a...
-          }
-          unfold subst_cset.
-          destruct_set_mem x {a}A; [exfalso;fsetdec|].
-          easy.
+      * assert (Hbnd : binds x0 (bind_typ (subst_ct x C (C1 # R))) (map (subst_cb x C) Δ ++ Γ)).
+        { replace (bind_typ (subst_ct x C (C1 # R)))
+             with (subst_cb x C (bind_typ (C1 # R)))
+             by reflexivity.
+          auto.
         }
-        eapply IHHsc...
+        eapply subcapt_var...
   - Case "subcapt_set".
     assert ((map (subst_cb x C) Δ ++ Γ) ⊢ₛ
                         (subst_cset x C (cset_set xs {}N b)) wf) as ?WF. {
       eapply wf_cset_subst_cb...
       constructor.
-      - intros y yIn.
-        enough ((Δ ++ [(x, bind_typ U)] ++ Γ) ⊢ₛ (`cset_fvar` y) wf) as HA. {
-          inversion HA...
-        }
-        specialize (H0 y yIn); simpl in H0...
-      - intros y yIn.
-        enough ((Δ ++ [(x, bind_typ U)] ++ Γ) ⊢ₛ (`cset_fvar` y) wf) as HA. {
-          inversion HA...
-        }
-        specialize (H0 y yIn); simpl in H0...
+      intros y yIn.
+      enough ((Δ ++ [(x, bind_typ U)] ++ Γ) ⊢ₛ (`cset_fvar` y) wf) as HA. {
+        inversion HA...
+      }
+      specialize (H0 y yIn); simpl in H0...
     }
     assert ((map (subst_cb x C) Δ ++ Γ) ⊢ₛ (subst_cset x C D) wf) as ?WF. {
       eapply wf_cset_subst_cb...
@@ -379,20 +324,6 @@ Proof with eauto using wf_env_subst_cb, wf_cset_subst_cb with fsetdec.
             unfold cset_union; csetsimpl...
           }
           eapply H1...
-        - cleanup_singleton_eq x y x0 x1.
-          replace (`cset_fvar` y) with (subst_cset x (cset_set ds {}N b__d) (`cset_fvar` y)).
-          2: {
-            unfold subst_cset; simpl.
-            destruct_set_mem x (singleton y); (trivial || exfalso;fsetdec).
-          }
-          replace (cset_set (ds `union` cs' `remove` x) {}N (b__d || b__c'))
-            with (subst_cset x (cset_set ds {}N b__d) (cset_set cs' {}N b__c')).
-          2: {
-            unfold subst_cset; simpl.
-            destruct_set_mem x cs'; [|exfalso;fsetdec].
-            unfold cset_union; csetsimpl...
-          }
-          eapply H1...
         - replace (`cset_fvar` y) with (subst_cset x (cset_set ds {}N b__d) (`cset_fvar` y)).
           2: {
             unfold subst_cset; simpl.
@@ -449,22 +380,8 @@ Proof with eauto using wf_env_subst_cb, wf_cset_subst_cb with fsetdec.
               destruct_set_mem x cs'; (trivial||exfalso;fsetdec).
             }
             eapply H1...
-        -- cleanup_singleton_eq x y x0 x1.
-            replace (`cset_fvar` y)
-              with (subst_cset x (cset_set ds {}N b__d) (`cset_fvar` y)).
-            2: {
-              unfold subst_cset; simpl.
-              destruct_set_mem x (`cset_fvar` y); (trivial || exfalso;fsetdec).
-            }
-            replace (cset_set cs' {}N b__c')
-              with (subst_cset x (cset_set ds {}N b__d) (cset_set cs' {}N b__c')).
-            2: {
-              unfold subst_cset; simpl.
-              destruct_set_mem x cs'; (trivial||exfalso;fsetdec).
-            }
-            eapply H1...
         -- replace (`cset_fvar` y)
-              with (subst_cset x (cset_set ds {}N b__d) (`cset_fvar` y)).
+            with (subst_cset x (cset_set ds {}N b__d) (`cset_fvar` y)).
             2: {
               unfold subst_cset; simpl.
               destruct_set_mem x (`cset_fvar` y); (trivial || exfalso;fsetdec).
@@ -511,7 +428,6 @@ Proof with eauto.
   intros ? ?.
   rewrite AtomSetFacts.union_iff in *.
   auto*.
-  fsetdec.
 Qed.
 
 Lemma subcapt_expansion : forall Γ C D1 D2,
@@ -532,7 +448,6 @@ Proof with eauto using wf_cset_union, wf_cset_atom_union with fsetdec.
     apply subcapt_in...
   - inversion HwfD2; simpl; subst...
   - eapply subcapt_var...
-  - eapply subcapt_tvar...
   - apply subcapt_set...
     + intros ? ?...
     + csetdec.
@@ -563,12 +478,8 @@ Proof with eauto with fsetdec.
     replace x with x0 by (clear - xIn; fsetdec)...
   - clear - xIn; fsetdec.
   - subst_mem_singleton xIn.
-    apply (subcapt_transitivity (typ_cv T))...
+    apply (subcapt_transitivity C1)...
     eapply subcapt_var...
-    eapply subcapt_reflexivity...
-  - subst_mem_singleton xIn.
-    apply (subcapt_transitivity (typ_cv T))...
-    eapply subcapt_tvar...
     eapply subcapt_reflexivity...
 Qed.
 
@@ -591,92 +502,59 @@ Proof with eauto using wf_cset_union with fsetdec.
   intros * WfΓ HscC1 HscC2.
   assert (Γ ⊢ₛ (C1 `u` C2) wf) by auto using wf_cset_union.
   generalize dependent C2.
-  dependent induction HscC1; intros C2 HscC2 WF__union...
-  - note (Γ ⊢ₛ C2 wf); csetsimpl.
+  dependent induction HscC1; intros C3 HscC3 WF__union...
+  - note (Γ ⊢ₛ C3 wf); csetsimpl.
     apply subcapt_set.
     + trivial...
     + intros y yIn.
       destruct_union_mem yIn.
       * subst_mem_singleton yIn.
         apply subcapt_in...
-      * applys subcapt_transitivity HscC2...
+      * applys subcapt_transitivity HscC3...
         apply subcapt_in...
         apply wf_concrete_cset...
-        2: fsetdec.
         intros z zIn...
-    + forwards: subcapt_universal_mem HscC2...
-  - note (Γ ⊢ₛ C2 wf); csetsimpl.
+    + forwards: subcapt_universal_mem HscC3...
+  - note (Γ ⊢ₛ C3 wf); csetsimpl.
     apply subcapt_set.
     + trivial...
     + intros y yIn.
-      applys subcapt_transitivity HscC2...
+      applys subcapt_transitivity HscC3...
       apply subcapt_in...
       apply wf_concrete_cset...
-      2: fsetdec.
       intros z zIn...
-    + forwards: subcapt_universal_mem HscC2...
-  - apply (subcapt_transitivity (typ_cv T `u` C2))...
-    assert (Γ ⊢ₛ (typ_cv T `u` C2) wf) as WfU by auto using wf_cset_union.
-    note (Γ ⊢ₛ C2 wf).
-    note (Γ ⊢ₛ (typ_cv T) wf).
-    rewrite <- H2 in WfU.
+    + forwards: subcapt_universal_mem HscC3...
+  - apply (subcapt_transitivity (C1 `u` C3))...
+    assert (Γ ⊢ₛ (C1 `u` C3) wf) as WfU by auto using wf_cset_union.
+    note (Γ ⊢ₛ C3 wf).
+    note (Γ ⊢ₛ C1 wf).
     csetsimpl.
     apply subcapt_set...
     2: csetdec.
     intros y yIn.
     destruct_union_mem yIn.
     + subst_mem_singleton yIn.
-      apply (subcapt_transitivity (typ_cv T))...
+      apply (subcapt_transitivity (cset_set fvars0 {}N univ0))...
       * eapply subcapt_var...
         eapply subcapt_reflexivity...
-      * rewrite <- H2.
-        apply subcapt_set...
+      * apply subcapt_set...
         2: csetdec.
         intros z zIn.
         apply subcapt_in...
         apply wf_concrete_cset...
-        2: fsetdec.
         intros w wIn...
     + apply subcapt_in...
       apply wf_concrete_cset...
-      2: fsetdec.
       intros z zIn...
-  - apply (subcapt_transitivity (typ_cv T `u` C2))...
-    assert (Γ ⊢ₛ (typ_cv T `u` C2) wf) as WfU by auto using wf_cset_union.
-    note (Γ ⊢ₛ C2 wf).
-    note (Γ ⊢ₛ (typ_cv T) wf).
-    rewrite <- H2 in WfU.
-    csetsimpl.
-    apply subcapt_set...
-    2: csetdec.
-    intros y yIn.
-    destruct_union_mem yIn.
-    + subst_mem_singleton yIn.
-      apply (subcapt_transitivity (typ_cv T))...
-      * eapply subcapt_tvar...
-        eapply subcapt_reflexivity...
-      * rewrite <- H2.
-        apply subcapt_set...
-        2: csetdec.
-        intros z zIn.
-        apply subcapt_in...
-        apply wf_concrete_cset...
-        2: fsetdec.
-        intros w wIn...
-    + apply subcapt_in...
-      apply wf_concrete_cset...
-      2: fsetdec.
-      intros z zIn...
-  - note (Γ ⊢ₛ C2 wf); csetsimpl.
+  - note (Γ ⊢ₛ C3 wf); csetsimpl.
     apply subcapt_set...
     + intros y yIn.
       destruct_union_mem yIn...
       apply (subcapt_transitivity (cset_set fvars {}N univ))...
       eapply subcapt_in...
       apply wf_concrete_cset...
-      2: fsetdec.
       intros z zIn...
-    + forwards: subcapt_universal_mem HscC2; csetdec...
+    + forwards: subcapt_universal_mem HscC3; csetdec...
 Qed.
 
 Lemma cset_union_symmetrical : forall C D,
@@ -700,398 +578,58 @@ Proof with eauto.
     apply subcapt_expansion...
 Qed.
 
+(* REVIEW: does not make sense anymore? *)
 Lemma subcapt_through_subst_tt : forall Γ P Q Δ X C D,
   (Δ ++ [(X, bind_sub Q)] ++ Γ) ⊢ wf ->
   (Δ ++ [(X, bind_sub Q)] ++ Γ) ⊢ₛ C <: D ->
-  (* TODO:
-      Q pure from wf_env
-      Q pure and P <: Q => P pure
-  *)
   Γ ⊢ P <: Q ->
-  (map (subst_tb X P) Δ ++ Γ) ⊢ₛ (subst_cset X (typ_cv P) C) <: (subst_cset X (typ_cv P) D).
+  (map (subst_tb X P) Δ ++ Γ) ⊢ₛ C <: D.
 Proof with eauto using wf_env_subst_tb, wf_cset_subst_tb, wf_typ_subst_tb with fsetdec.
-  intros * Hwf Hsc Hsub.
-  assert ((map (subst_tb X P) Δ ++ Γ) ⊢ wf).
-  { eapply wf_env_subst_tb...
-    admit.
+  intros * WfEnv Subcapt Sub.
+  assert (PureQ : pure_type Q).
+  { eapply wf_env_tail in WfEnv.
+    inversion WfEnv...
   }
+  assert (PureP : pure_type P) by (apply (proj2 (sub_pure_type _ _ _ Sub) PureQ)).
+  assert ((map (subst_tb X P) Δ ++ Γ) ⊢ wf).
+  { eapply wf_env_subst_tb... }
   generalize dependent P.
-  dependent induction Hsc; intros P Hsub Henv.
-  - assert ((map (subst_tb X P) Δ ++ Γ) ⊢ₛ (subst_cset X (typ_cv P) C) wf) as ?WF...
-    assert ((map (subst_tb X P) Δ ++ Γ) ⊢ₛ
-                       (subst_cset X (typ_cv P) (cset_set xs {}N true)) wf) as ?WF...
-    cbv [subst_cset] in *.
-    destruct_set_mem X xs.
-    + assert ((Δ ++ [(X, bind_sub Q)] ++ Γ) ⊢ P wf) as HA. {
-        note (([(X, bind_sub Q)] ++ Γ) ⊢ wf) by eauto...
-        rewrite_env (∅ ++ (Δ ++ [(X, bind_sub Q)]) ++ Γ).
-        apply wf_typ_weakening; simpl_env...
-      }
-      forwards: cv_wf HA.
-      inversion HA; subst; simpl in *; csetsimpl; apply subcapt_universal...
-    + apply subcapt_universal...
-  - assert ((map (subst_tb X P) Δ ++ Γ) ⊢ₛ (subst_cset X (typ_cv P) (`cset_fvar` x)) wf) as ?WF...
-    assert ((map (subst_tb X P) Δ ++ Γ) ⊢ₛ
-                       (subst_cset X (typ_cv P) (cset_set xs {}N b)) wf) as ?WF...
-    unfold subst_cset in *.
-    destruct_set_mem X {x}A.
-    + destruct_set_mem X xs.
-      2: exfalso; fsetdec.
-      assert ((Δ ++ [(X, bind_sub Q)] ++ Γ) ⊢ₛ (typ_cv P) wf) as HA. {
-        note (([(X, bind_sub Q)] ++ Γ) ⊢ wf) by eauto...
-        rewrite_env (∅ ++ (Δ ++ [(X, bind_sub Q)]) ++ Γ).
-        apply wf_cset_weakening; simpl_env; [apply cv_wf|]...
-      }
-      inversion HA; subst; csetsimpl.
-      replace (xs `union` singleton x `remove` X) with xs by fsetdec.
-      rename select (_ = typ_cv P) into EQ.
-      rewrite <- EQ in WF0; csetsimpl in WF0.
-      apply subcapt_set...
-      * intros y yIn.
-        apply subcapt_in...
-        eapply wf_cset_singleton_by_mem...
-      * csetdec.
-    + destruct_set_mem X xs.
-      2: {
-        apply subcapt_in...
-      }
-      assert ((Δ ++ [(X, bind_sub Q)] ++ Γ) ⊢ₛ (typ_cv P) wf) as HA. {
-        note (([(X, bind_sub Q)] ++ Γ) ⊢ wf) by eauto...
-        rewrite_env (∅ ++ (Δ ++ [(X, bind_sub Q)]) ++ Γ).
-        apply wf_cset_weakening; simpl_env; [apply cv_wf|]...
-      }
-      inversion HA; subst; csetsimpl.
-      rename select (_ = typ_cv P) into EQ.
-      rewrite <- EQ in WF0; csetsimpl in WF0.
-      apply subcapt_in...
-  - assert ((map (subst_tb X P) Δ ++ Γ) ⊢ₛ (subst_cset X (typ_cv P) D) wf)...
-    inversion select (_ ⊢ₛ D wf); repeat subst. (* so apparently subst isn't idempotent *)
-    unfold subst_cset in *.
-    find_and_destroy_set_mem; [exfalso;fsetdec|].
-    find_and_destroy_set_mem.
-    + assert (Γ ⊢ₛ (typ_cv P) wf) as HA; [|inversion HA; subst]. {
-        apply cv_wf...
-      }
-      rename select (_ = typ_cv P) into EQ.
-      rewrite <- EQ in H1.
-      csetsimpl.
-      apply subcapt_universal...
-    + apply subcapt_universal...
-  - unfold subst_cset at 1.
-    destruct_set_mem X {x}A.
-    + assert (x = X) by fsetdec; subst.
-      assert (binds X (bind_sub Q) (Δ ++ [(X, bind_sub Q)] ++ Γ)) as HA by auto.
-      forwards: binds_unique (bind_typ T) (bind_sub Q)...
-      congruence.
-    + assert (x <> X) by fsetdec.
-      binds_cases H.
-      * specialize (IHHsc X Δ Q Γ ltac:(trivial) ltac:(trivial) ltac:(trivial)).
-        forwards: wf_typ_from_binds_typ H...
-        eapply subcapt_var with (T := T)...
-        replace (typ_cv T) with (subst_cset X (typ_cv P) (typ_cv T)).
-        2: {
-          symmetry; apply subst_cset_fresh.
-          assert (X ∉ dom Γ) as HA. {
-            assert (ok (Δ ++ [(X, bind_sub Q)] ++ Γ)) as HA by auto.
-            apply ok_tail in HA.
-            inversion HA...
-          }
-          forwards: notin_fv_wf_typ H1 HA.
-          destruct T; simpl in *; try fsetdec.
-          destruct v...
-        }
-        apply IHHsc...
-      * assert (binds x (bind_typ (subst_tt X P T)) (map (subst_tb X P) Δ ++ Γ)) as HBnd by auto.
-        eapply subcapt_var...
-        replace (typ_cv (subst_tt X P T))
-          with (subst_cset X (typ_cv P) (typ_cv T)).
-        1: eapply IHHsc...
-        1: {
-          destruct T; unfold subst_cset; simpl...
-          destruct v; simpl...
-          2-6: destruct_if; [ exfalso; csetdec | reflexivity ].
-          destruct (a == X); destruct_set_mem X {a}A; try (exfalso;fsetdec).
-          2: simpl...
-          note (Γ ⊢ P wf); simpl; unfold cset_union; csetdec.
-        }
-  - unfold subst_cset at 1.
-    destruct_set_mem X (singleton x).
-    + assert (x = X) by fsetdec; subst.
-      assert (binds X (bind_sub Q) (Δ ++ [(X, bind_sub Q)] ++ Γ)) as HBnd by auto.
-      forwards EQ: binds_unique H HBnd.
-      inversion EQ; subst.
-      assert (Γ ⊢ P wf) as WfP by eauto.
-      assert (Γ ⊢ Q wf) as WfQ by eauto.
-      assert (X ∉ dom Γ) as HA. {
-        assert (ok (Δ ++ [(X, bind_sub Q)] ++ Γ)) as HA by auto.
-        apply ok_tail in HA.
-        inversion HA...
-      }
-      forwards: notin_fv_wf_typ WfP HA.
-      forwards: notin_fv_wf_typ WfQ HA.
-      replace (typ_cv P `u` cset_set ({X}A `\`A X) {}N false)
-        with (typ_cv P) by (destruct (typ_cv P); csetdec).
-      replace (typ_cv P) with (subst_cset X (typ_cv P) (typ_cv P)) at 1.
-      2: {
-        symmetry.
-        apply subst_cset_fresh.
-        destruct P; simpl in *; try fsetdec.
-        destruct v...
-      }
-      apply (subcapt_transitivity (subst_cset X (typ_cv P) (typ_cv Q)))...
-      eenough (Γ ⊢ₛ _ <: _) as HE. {
-        rewrite_env (∅ ++ (map (subst_tb X P) Δ ++ Γ)).
-        apply subcapt_weakening; simpl_env...
-      }
-      do 2 erewrite <- typ_cv_subst_ct_correspondence by fsetdec.
-      do 2 erewrite <- subst_ct_fresh by fsetdec.
-      apply sub_implies_subcapt...
-    + assert (x <> X) by fsetdec.
-      binds_cases H.
-      * specialize (IHHsc X Δ Q Γ ltac:(trivial) ltac:(trivial) ltac:(trivial)).
-        forwards: wf_typ_from_binds_sub H...
-        eapply subcapt_tvar with (T := T)...
-        replace (typ_cv T) with (subst_cset X (typ_cv P) (typ_cv T)).
-        2: {
-          symmetry; apply subst_cset_fresh.
-          assert (X ∉ dom Γ) as HA. {
-            assert (ok (Δ ++ [(X, bind_sub Q)] ++ Γ)) as HA by auto.
-            apply ok_tail in HA.
-            inversion HA...
-          }
-          forwards: notin_fv_wf_typ H1 HA.
-          destruct T; simpl in *; try fsetdec.
-          destruct v...
-        }
-        apply IHHsc...
-      * assert (binds x (bind_sub (subst_tt X P T)) (map (subst_tb X P) Δ ++ Γ)) as HBnd by auto.
-        eapply subcapt_tvar...
-        replace (typ_cv (subst_tt X P T))
-          with (subst_cset X (typ_cv P) (typ_cv T)).
-        1: eapply IHHsc...
-        1: {
-          destruct T; unfold subst_cset; simpl...
-          destruct v; simpl.
-          2-6: destruct_if; [ exfalso; csetdec | reflexivity ].
-          destruct (a == X); destruct_set_mem X {a}A; try (exfalso;fsetdec).
-          2: simpl...
-          note (Γ ⊢ P wf); simpl; unfold cset_union; csetdec.
-        }
-  - assert ((map (subst_tb X P) Δ ++ Γ) ⊢ₛ
-                       (subst_cset X (typ_cv P) (cset_set xs {}N b)) wf) as ?WF. {
-      eapply wf_cset_subst_tb...
-      constructor.
-      - intros y yIn.
-        enough ((Δ ++ [(X, bind_sub Q)] ++ Γ) ⊢ₛ (`cset_fvar` y) wf) as HA. {
-          inversion HA...
-        }
-        specialize (H0 y yIn); simpl in H0...
-      - intros y yIn.
-        enough ((Δ ++ [(X, bind_sub Q)] ++ Γ) ⊢ₛ (`cset_fvar` y) wf) as HA. {
-          inversion HA...
-        }
-        specialize (H0 y yIn); simpl in H0...
-    }
-    assert ((map (subst_tb X P) Δ ++ Γ) ⊢ₛ
-                       (subst_cset X (typ_cv P) D) wf) as ?WF. {
-      eapply wf_cset_subst_tb...
-    }
-
-    unfold subst_cset at 1.
-    unfold subst_cset in WF.
-    destruct_set_mem X xs.
-    2: {
-      apply subcapt_set; trivial.
-      - intros y yIn.
-        assert (X <> y) by notin_solve.
-        replace (`cset_fvar` y) with (subst_cset X (typ_cv P) (`cset_fvar` y))...
-        unfold subst_cset.
-        destruct_set_mem X (singleton y)...
-        exfalso; fsetdec.
-      - (* Should we have a lemma that `cset_uvar` is not affected by subst? *)
-        (* Looking at that chain, we probably should. *)
-        destruct D; unfold subst_cset; destruct_if; destruct P; simpl; csetdec.
-        destruct v...
-    }
-
-    unfold AtomSet.F.For_all in H0.
-
-    inversion H; subst.
-    assert ((Δ ++ [(X, bind_sub Q)] ++ Γ) ⊢ₛ (typ_cv P) wf) as HA. {
-      note (([(X, bind_sub Q)] ++ Γ) ⊢ wf) by eauto...
-      rewrite_env (∅ ++ (Δ ++ [(X, bind_sub Q)]) ++ Γ).
-      apply wf_cset_weakening; simpl_env; [apply cv_wf|]...
-    }
-    inversion HA; subst.
-
-    rename fvars into cs', univ into b__c', fvars0 into ds, univ0 into b__d.
-    unfold subst_cset in WF0 |- *.
-    destruct_set_mem X cs'.
-    + rename select (_ = typ_cv P) into EQ.
-      rewrite <- EQ in WF, WF0.
-      csetsimpl.
-      apply subcapt_set; trivial.
-      2: csetdec.
-      intros y yIn.
-      destruct_union_mem yIn. {
-        apply subcapt_in...
-        eapply wf_cset_singleton_by_mem...
-      }
-
-      specialize (H0 y ltac:(fsetdec)); simpl in H0.
-      Local Ltac cleanup_singleton_eq' x y x0 :=
-        let HA := fresh "HA" in
-        let xEQ := fresh x "EQ" in
-        rename x into xEQ;
-        assert (x0 `in` singleton x0) as HA by fsetdec;
-        rewrite xEQ in HA;
-        assert (x0 = y) by fsetdec;
-        subst;
-        clear xEQ HA.
-
-      dependent induction H0.
-      * csetsimpl.
-        apply subcapt_universal...
-        applys wf_cset_singleton_by_mem (ds `u`A xs `\`A X)...
-      * cleanup_singleton_eq' x y x0.
-        apply subcapt_in...
-        applys wf_cset_singleton_by_mem (ds `u`A xs `\`A X)...
-      * cleanup_singleton_eq' x y x0.
-        rename select (_ = typ_cv P) into EQ.
-        replace (`cset_fvar` y) with (subst_cset X (typ_cv P) (`cset_fvar` y)).
-        2: {
-          unfold subst_cset; simpl.
-          destruct_set_mem X (singleton y); (trivial || exfalso;fsetdec).
-        }
-        replace (cset_set (ds `union` cs' `remove` X) {}N (b__d || b__c'))
-          with (subst_cset X (typ_cv P) (cset_set cs' {}N b__c')).
-        2: {
-          unfold subst_cset; simpl.
-          destruct_set_mem X cs'; [|exfalso;fsetdec].
-          rewrite <- EQ.
-          csetsimpl...
-        }
-        (* rewrite EQ. *)
-        eapply H1...
-      * cleanup_singleton_eq' x y x0.
-        rename select (_ = typ_cv P) into EQ.
-        replace (`cset_fvar` y) with (subst_cset X (typ_cv P) (`cset_fvar` y)).
-        2: {
-          unfold subst_cset; simpl.
-          destruct_set_mem X (singleton y); (trivial || exfalso;fsetdec).
-        }
-        replace (cset_set (ds `union` cs' `remove` X) {}N (b__d || b__c'))
-          with (subst_cset X (typ_cv P) (cset_set cs' {}N b__c')).
-        2: {
-          unfold subst_cset; simpl.
-          destruct_set_mem X cs'; [|exfalso;fsetdec].
-          rewrite <- EQ.
-          unfold cset_union; csetsimpl...
-        }
-        eapply H1...
-      * rename select (_ = typ_cv P) into EQ.
-        replace (`cset_fvar` y) with (subst_cset X (typ_cv P) (`cset_fvar` y)).
-        2: {
-          unfold subst_cset; simpl.
-          destruct_set_mem X (singleton y); (trivial || exfalso;fsetdec).
-        }
-        replace (cset_set (ds `union` cs' `remove` X) {}N (b__d || b__c'))
-          with (subst_cset X (typ_cv P) (cset_set cs' {}N b__c')).
-        2: {
-          unfold subst_cset; simpl.
-          destruct_set_mem X cs'; [|exfalso;fsetdec].
-          rewrite <- EQ.
-          csetsimpl...
-        }
-        eapply H1...
-    + csetsimpl.
-      rename select (_ = typ_cv P) into EQ.
-      apply subcapt_set; trivial.
-      2: {
-        forwards SpH1: H1 X X Δ Q Γ...
-        rewrite <- EQ in SpH1.
-        unfold subst_cset in SpH1.
-        find_and_destroy_set_mem; [|exfalso;fsetdec].
-        find_and_destroy_set_mem; [exfalso;fsetdec|].
-        csetsimpl in SpH1.
-        destr_bool.
-        inversion SpH1; subst; easy.
-      }
-      intros y yIn.
-      destruct_set_mem y (xs `remove` X).
-      * specialize (H0 y ltac:(fsetdec)); simpl in H0.
-        dependent induction H0.
-        -- apply subcapt_universal...
-           rewrite <- EQ in WF; csetsimpl; applys wf_cset_singleton_by_mem yIn...
-        -- cleanup_singleton_eq' x y x0.
-           apply subcapt_in...
-           replace (`cset_fvar` y) with (subst_cset X (typ_cv P) (`cset_fvar` y)).
-           eapply wf_cset_subst_tb...
-           symmetry.
-           apply subst_cset_fresh...
-        -- cleanup_singleton_eq' x y x0.
-           replace (`cset_fvar` y) with (subst_cset X (typ_cv P) (`cset_fvar` y)).
-           2: {
-             unfold subst_cset; simpl.
-             destruct_set_mem X (`cset_fvar` y); (trivial || exfalso;fsetdec).
-           }
-           replace (cset_set cs' {}N b__c') with (subst_cset X (typ_cv P) (cset_set cs' {}N b__c')).
-           2: {
-             unfold subst_cset; simpl.
-             destruct_set_mem X cs'; (trivial||exfalso;fsetdec).
-           }
-           eapply H1...
-        -- cleanup_singleton_eq' x y x0.
-           replace (`cset_fvar` y) with (subst_cset X (typ_cv P) (`cset_fvar` y)).
-           2: {
-             unfold subst_cset; simpl.
-             destruct_set_mem X (`cset_fvar` y); (trivial || exfalso;fsetdec).
-           }
-           replace (cset_set cs' {}N b__c') with (subst_cset X (typ_cv P) (cset_set cs' {}N b__c')).
-           2: {
-             unfold subst_cset; simpl.
-             destruct_set_mem X cs'; (trivial||exfalso;fsetdec).
-           }
-           eapply H1...
-        -- replace (`cset_fvar` y) with (subst_cset X (typ_cv P) (`cset_fvar` y)).
-           2: {
-             unfold subst_cset; simpl.
-             destruct_set_mem X (`cset_fvar` y); (trivial || exfalso;fsetdec).
-           }
-           replace (cset_set cs' {}N b__c') with (subst_cset X (typ_cv P) (cset_set cs' {}N b__c')).
-           2: {
-             unfold subst_cset; simpl.
-             destruct_set_mem X cs'; (trivial||exfalso;fsetdec).
-           }
-           eapply H1...
-      * destruct_union_mem yIn.
-        2: exfalso...
-        rename H1 into H1'.
-        forwards H1: (>> H1' X XIn X Δ Q Γ)...
-        move H1 before H1'; clear H1'.
-        unfold subst_cset at 1 in H1.
-        destruct_set_mem X {X}A; [|exfalso;fsetdec].
-
-        unfold subst_cset at 1 in H1.
-        destruct_set_mem X cs'; [exfalso;fsetdec|].
-
-        rewrite <- EQ in H1.
-        csetsimpl.
-
-        replace (ds `u`A {X}A `\`A X) with ds in H1 by fsetdec.
-
-        enough ((map (subst_tb X P) Δ ++ Γ) ⊢ₛ
-                         (`cset_fvar` y) <:
-                         (cset_set ds {}N b__d)) as HAA. {
-          eapply subcapt_transitivity...
-        }
-        eapply subcapt_in...
-        forwards (? & ?): subcapt_regular H1.
-        inversion select (_ ⊢ₛ (cset_set ds _ _) wf); subst...
-        eapply wf_cset_singleton_by_mem...
-        repeat rewrite dom_concat in *; repeat rewrite dom_map in *; simpl in *.
-        admit.
-Admitted.
+  dependent induction Subcapt; intros P Sub PureP WfEnvSubst.
+  - Case "subcapt_univeral".
+    apply subcapt_universal.
+    + apply wf_concrete_cset.
+      inversion select (_ ⊢ₛ cset_set xs _ _ wf); subst.
+      intros x xIn.
+      rename select (allbound _ _) into AllBound.
+      destruct (AllBound x xIn) as [T Binds].
+      binds_cases Binds.
+      * exists T.
+        apply binds_tail...
+      * exists (subst_tt X P T).
+        replace (bind_typ (subst_tt X P T))
+          with (subst_tb X P (bind_typ T))
+            by reflexivity.
+        apply binds_head...
+    + eapply wf_cset_subst_tb...
+  - Case "subcapt_in".
+    apply subcapt_set...
+    intros y yIn; assert (y = x) by fsetdec; subst; clear yIn.
+    eapply subcapt_in...
+  - Case "subcapt_in_univ".
+    apply subcapt_in_univ...
+  - Case "subcapt_var".
+    rename select (binds x _ _) into Binds.
+    binds_cases Binds...
+    eapply subcapt_var with (R := subst_tt X P R)...
+    replace (bind_typ (C1 # subst_tt X P R))
+       with (subst_tb X P (bind_typ (C1 # R)))
+         by reflexivity.
+    apply binds_head, binds_map...
+  - Case "subcapt_set".
+    apply subcapt_set...
+    intros y yIn.
+    eapply H1...
+Qed.
 
 (* (* ********************************************************************** *) *)
 (* (** ** Narrowing and transitivity (3) *) *)
@@ -1140,7 +678,6 @@ Proof with eauto with fsetdec.
       destruct (AtomSet.F.union_1 yIn).
       * assert (y = x0) by fsetdec; subst...
       * apply wf_concrete_cset...
-        2: fsetdec.
         intros z zIn...
     + csetdec.
   - csetsimpl.
@@ -1148,7 +685,6 @@ Proof with eauto with fsetdec.
     intros y yIn.
     apply subcapt_in...
     apply wf_concrete_cset...
-    2: fsetdec.
     intros z zIn...
   - csetsimpl.
     apply subcapt_set...
@@ -1158,7 +694,6 @@ Proof with eauto with fsetdec.
     2: {
       apply subcapt_in...
       apply wf_concrete_cset...
-      2: fsetdec.
       intros z zIn...
     }
     rename select (y `in`A _) into yIn.
@@ -1169,7 +704,6 @@ Proof with eauto with fsetdec.
     + intros z zIn.
       apply subcapt_in...
       apply wf_concrete_cset...
-      2: fsetdec.
       intros w wIn...
     + csetdec.
   - csetsimpl.
@@ -1180,29 +714,6 @@ Proof with eauto with fsetdec.
     2: {
       apply subcapt_in...
       apply wf_concrete_cset...
-      2: fsetdec.
-      intros z zIn...
-    }
-    rename select (y `in`A _) into yIn.
-    apply AtomSetFacts.singleton_iff in yIn; symmetry in yIn; subst.
-    eapply subcapt_tvar...
-    apply (subcapt_transitivity (cset_set ds {}N univ1))...
-    apply subcapt_set...
-    + intros z zIn.
-      apply subcapt_in...
-      apply wf_concrete_cset...
-      2: fsetdec.
-      intros w wIn...
-    + csetdec.
-  - csetsimpl.
-    apply subcapt_set...
-    2: csetdec.
-    intros y yIn.
-    destruct_union_mem yIn.
-    2: {
-      apply subcapt_in...
-      apply wf_concrete_cset...
-      2: fsetdec.
       intros z zIn...
     }
     apply (subcapt_transitivity (cset_set ds {}N univ1))...
@@ -1211,7 +722,6 @@ Proof with eauto with fsetdec.
     + intros z zIn.
       apply subcapt_in...
       apply wf_concrete_cset...
-      2: fsetdec.
       intros w wIn...
     + csetdec.
 Qed.
@@ -1227,49 +737,26 @@ Proof with eauto.
   intros * Ok WfE Wf1 Wf2 Sc.
   dependent induction Sc...
   - inversion Wf1; subst; cbv [allbound] in *...
-    specialize (H3 x ltac:(fsetdec)) as [Tx Hbinds].
-    destruct Hbinds...
-    * assert (Tx = T). {
-        eapply binds_weaken in H0...
-        unshelve epose proof (binds_unique _ _ _ _ H H0)...
-        inversion H1...
-      }
-      subst...
-      eapply subcapt_var...
-      eapply IHSc...
-      apply cv_wf...
-      eapply wf_typ_from_binds_typ...
-    * exfalso.
-      eapply binds_weaken in H0...
-      unshelve epose proof (binds_unique _ _ _ _ H H0)...
-      inversion H1...
-  - inversion Wf1; subst; cbv [allbound] in *...
-    specialize (H3 x ltac:(fsetdec)) as [Tx Hbinds].
-    destruct Hbinds...
-    * exfalso.
-      eapply binds_weaken in H0...
-      unshelve epose proof (binds_unique _ _ _ _ H H0)...
-      inversion H1...
-    * assert (Tx = T). {
-        eapply binds_weaken in H0...
-        unshelve epose proof (binds_unique _ _ _ _ H H0)...
-        inversion H1...
-      }
-      subst...
-      eapply subcapt_tvar...
-      eapply IHSc...
-      apply cv_wf...
-      eapply wf_typ_from_binds_sub...
+    rename select (forall x0, _ ∈ {x}A -> _) into Hb.
+    specialize (Hb x ltac:(fsetdec)) as [Tx Hbinds].
+    assert (Tx = C1 # R). {
+      eapply binds_weaken in Hbinds...
+      unshelve epose proof (binds_unique _ _ _ _ H Hbinds)...
+      inversion H0...
+    }
+    subst...
+    eapply subcapt_var...
+    eapply IHSc...
+    enough (Hwf: (Δ ++ Γ) ⊢ (C1 # R) wf) by (inversion Hwf; auto).
+    eapply wf_typ_from_binds_typ...
   - destruct D as [fvD bvD univD]; subst...
     inversion H; subst...
     apply subcapt_set...
-    * intros a aInXs.
-      eapply H1...
-      inversion Wf1; subst.
-      eapply wf_concrete_cset...
-      -- intros z zIn; assert (z = a) by (clear - zIn; fsetdec); subst...
-      -- rewrite dom_concat in H9 |- *.
-         fsetdec.
+    intros a aInXs.
+    eapply H1...
+    inversion Wf1; subst.
+    eapply wf_concrete_cset...
+    intros z zIn; assert (z = a) by (clear - zIn; fsetdec); subst...
 Qed.
 
 Lemma subcapt_widening_univ : forall X Δ Γ P Q C,
@@ -1303,6 +790,7 @@ Qed.
 (* TODO: move to CCsub_Lemmas.v
 typ_cv_free_never_universal *)
 
+(* TODO: remove? if typing_through_subst_ve is indeed not useful
 Lemma subcapt_univ_through_subst_cb : forall Δ Γ x u P T,
   (Δ ++ [(x, bind_typ (exp_cv u # P))] ++ Γ) ⊢ₛ (typ_cv T) wf ->
   (map (subst_cb x (exp_cv u)) Δ ++ Γ) ⊢ₛ {*} <: (typ_cv (subst_ct x (exp_cv u) T)) ->
@@ -1324,36 +812,4 @@ Proof with eauto.
     admit.
   + apply subcapt_in_univ; trivial.
 Admitted.
-
-Lemma subcapt_univ_through_subst_tb : forall Δ Γ Z P T,
-  (Δ ++ [(Z, bind_sub P)] ++ Γ) ⊢ T wf ->
-  Γ ⊢ P wf ->
-  (map (subst_tb Z P) Δ ++ Γ) ⊢ₛ {*} <: typ_cv (subst_tt Z P T) ->
-  (Δ ++ [(Z, bind_sub P)] ++ Γ) ⊢ₛ {*} <: typ_cv T
-    \/ (Z ∈ (`cset_fvars` (typ_cv T))
-          /\ Γ ⊢ₛ {*} <: typ_cv P).
-Proof with eauto.
-  intros * WfT WfP ScUniv.
-  forwards: univ_supercapt_inversion ScUniv.
-  inversion WfT; subst; simpl in *; simpl_env in *; try congruence.
-  - destruct (X == Z); subst.
-    + right; split.
-      * fsetdec.
-      * apply subcapt_in_univ; trivial.
-        eapply cv_wf...
-    + simpl in *; congruence.
-  - inversion H0; subst.
-    destruct univ.
-    1: {
-      left.
-      apply subcapt_in_univ; trivial.
-    }
-    unfold subst_cset in H.
-    find_and_destroy_set_mem; try congruence.
-    assert (Γ ⊢ₛ (typ_cv P) wf) as WfCvP by (eapply cv_wf; eauto).
-    inversion WfCvP; subst.
-    rename select (_ = typ_cv P) into EQ; rewrite <- EQ in *.
-    unfold cset_union in H.
-    destruct univ; simpl in *; try congruence.
-    right; split...
-Qed.
+*)
