CCsub_Typing.v
@@ -1,5 +1,6 @@
 Require Import Coq.Program.Equality.
 Require Import TaktikZ.
+Require Import LibTactics.
 Require Export CCsub_Hints.
 Require Import CCsub_Subcapt.
 Require Import CCsub_Subtyping.
@@ -7,140 +8,143 @@ Require Import CCsub_Subtyping.
 (* ********************************************************************** *)
 (** * #<a name="typing"></a># Properties of typing *)
 
-
 (* ********************************************************************** *)
 (** ** Weakening (5) *)
-Lemma typing_weakening : forall E F G e T,
-  typing (G ++ E) e T ->
-  wf_env (G ++ F ++ E) ->
-  typing (G ++ F ++ E) e T.
+Lemma typing_weakening : forall Γ Θ Δ e T,
+  (Δ ++ Γ) ⊢ e : T ->
+  (Δ ++ Θ ++ Γ) ⊢ wf ->
+  (Δ ++ Θ ++ Γ) ⊢ e : T.
 Proof with simpl_env;
            eauto using wf_typ_weakening,
-                       wf_typ_in_weakening,
                        wf_typ_from_wf_env_typ,
                        wf_typ_from_wf_env_sub,
                        sub_weakening,
                        subcapt_weakening.
   intros * Typ.
-  remember (G ++ E).
-  generalize dependent G.
-  induction Typ; intros G EQ Ok; subst...
+  remember (Δ ++ Γ).
+  generalize dependent Δ.
+  induction Typ; intros Δ EQ Ok; subst...
   - Case "typing_abs".
     pick fresh X and apply typing_abs...
-    + lapply (H0 X); [intros K | auto].
-      simpl_env in *.
-      rewrite <- concat_assoc.
-      eapply wf_typ_weakening.
-      * apply K.
-      * trivial...
-      * clear; fsetdec.
-      * clear; fsetdec.
-    + lapply (H1 X); [intros K | auto].
-      simpl_env in *.
-      rewrite <- concat_assoc.
-      apply (H2 X)...
+    lapply (H0 X); [intros K | auto].
+    simpl_env in *.
+    rewrite <- concat_assoc.
+    apply H1...
   - Case "typing_let".
     pick fresh X and apply typing_let...
     lapply (H X); [intros K | auto].
     simpl_env in *.
     rewrite <- concat_assoc.
     apply (H0 X)...
-    constructor...
-    apply wf_typ_in_weakening...
-    applys typing_regular Typ.
+    apply wf_env_typ...
+    destructs typing_regular Typ as [WfEnv [Expr WfTyp]].
+    constructor.
+    + apply wf_cset_weakening... 
+    + apply wf_typ_weakening...
+      inversion WfTyp...
+    + enough (Typ' : type (C1 # T1)) by (inversion Typ'; subst; [ inversion H1 | auto ]).
+      eapply type_from_wf_typ, WfTyp.
   - Case "typing_tabs".
     pick fresh X and apply typing_tabs...
-    + lapply (H0 X); [intros K | auto].
-      simpl_env in *.
-      rewrite <- concat_assoc.
-      eapply wf_typ_weakening.
-      * apply K.
-      * trivial...
-      * clear; fsetdec.
-      * clear; fsetdec.
-    + lapply (H1 X); [intros K | auto].
-      simpl_env in *.
-      rewrite <- concat_assoc.
-      apply (H2 X)...
+    lapply (H1 X); [intros K | auto].
+    simpl_env in *.
+    rewrite <- concat_assoc.
+    apply H2...
+  - Case "typing_box".
+    apply typing_box...
+    simpl_env in H.
+    fsetdec.
+  - Case "typing_unbox".
+    apply typing_unbox...
+    apply wf_cset_weakening... 
 Qed.
 
 
 (************************************************************************ *)
 (** ** Narrowing for typing (7) *)
 
-Lemma typing_narrowing : forall Q E F X P e T,
-  sub E P Q ->
-  typing (F ++ [(X, bind_sub Q)] ++ E) e T ->
-  typing (F ++ [(X, bind_sub P)] ++ E) e T.
-Proof with eauto using wf_env_narrowing, wf_typ_narrowing, sub_narrowing, subcapt_narrowing.
+Lemma typing_narrowing : forall Q Δ Γ X P e T,
+  Γ ⊢ P <: Q ->
+  (Δ ++ [(X, bind_sub Q)] ++ Γ) ⊢ e : T ->
+  (Δ ++ [(X, bind_sub P)] ++ Γ) ⊢ e : T.
+Proof with eauto using wf_env_narrowing, wf_typ_ignores_sub_bindings, sub_narrowing, subcapt_narrowing.
   intros * PsubQ Typ.
-  remember (F ++ [(X, bind_sub Q)] ++ E).
-  generalize dependent F.
-  induction Typ; intros F EQ; subst...
+  assert (PureP : pure_type P).
+  { enough (PureQ : pure_type Q) by (applys sub_pure_type PsubQ; eauto* ).
+    forwards (WfEnv & _): typing_regular Typ.
+    apply wf_env_tail in WfEnv.
+    inversion WfEnv...
+  }
+  assert (WfEnv : wf_env (Δ ++ [(X, bind_sub P)] ++ Γ)). {
+    apply wf_env_narrowing with (V := Q)...
+    applys typing_regular Typ.
+  }
+  remember (Δ ++ [(X, bind_sub Q)] ++ Γ).
+  generalize dependent Δ.
+  induction Typ; intros Δ EQ WfEnv; subst.
   - Case "typing_var".
     binds_cases H0...
-    constructor...
-  - Case "typing_var".
-    binds_cases H0...
-    eapply typing_var...
   - Case "typing_abs".
-    assert (wf_env (F ++ [(X, bind_sub P)] ++ E)). {
-      pick fresh y for L.
-      forwards (P0 & _): typing_regular (H1 y Fr).
-      inversion P0; subst...
-    }
     pick fresh y and apply typing_abs...
-    + rewrite_parenthesise_binding.
-      simpl_env in H0...
-      eapply wf_typ_narrowing_base; simpl_env...
-    + rewrite <- concat_assoc.
-      apply H2...
+    rewrite <- concat_assoc.
+    apply H1...
+    econstructor...
+  - Case "typing_app".
+    eapply typing_app...
   - Case "typing_let".
-    assert (wf_env (F ++ [(X, bind_sub P)] ++ E)). {
-      pick fresh y for L.
-      forwards (P0 & _): typing_regular (H y Fr).
-      inversion P0; subst...
-    }
     pick fresh y and apply typing_let...
     rewrite_parenthesise_binding.
-    simpl_env in H0...
+    apply H0...
+    apply wf_env_typ...
+    apply wf_typ_ignores_sub_bindings with (V := Q).
+    applys typing_regular Typ.
   - Case "typing_tabs".
-    assert (wf_env (F ++ [(X, bind_sub P)] ++ E)). {
-      pick fresh y for L.
-      forwards (P0 & _): typing_regular (H1 y Fr).
-      inversion P0; subst...
-    }
     pick fresh Y and apply typing_tabs...
-    + rewrite_parenthesise_binding.
-      simpl_env in H0...
-      eapply wf_typ_narrowing_base; simpl_env...
-    + rewrite <- concat_assoc.
-      apply H2...
+    rewrite <- concat_assoc.
+    apply H2...
+    apply wf_env_sub...
+  - Case "typing_tapp".
+    eapply typing_tapp...
+  - Case "typing_box".
+    apply typing_box...
+    simpl_env in *; assumption.
+  - Case "typing_unbox".
+    apply typing_unbox...
+    eapply wf_cset_narrowing...
+  - Case "typing_sub".
+    apply typing_sub with (S := S)... 
 Qed.
 
+(* REVIEW: not needed anymore: we have a strict distinction between pure and capt type
+           even though the raw syntax encompasses both 
 Inductive syn_cat_agree : typ -> typ -> Prop :=
 | syn_cat_agree_tvar : forall (X Y : atom),
     syn_cat_agree X Y
 | syn_cat_agree_concrete : forall C P D U,
-    syn_cat_agree (typ_capt C P) (typ_capt D U).
+    syn_cat_agree (typ_capt C P) (typ_capt D U). *)
 
-Lemma sub_of_tvar : forall E P (X : atom),
-  sub E P X ->
+Lemma sub_of_tvar : forall Γ P (X : atom),
+  Γ ⊢ P <: X ->
   exists (Y : atom), P = Y.
 Proof.
-  intros * H.
-  dependent induction H...
+  intros * Sub.
+  assert (PureP : pure_type P).
+  { applys sub_pure_type Sub.
+    constructor.
+  }
+  dependent induction Sub...
   * exists X; trivial.
-  * exists X0; trivial.
+  * inversion PureP.
 Qed.
 
-Lemma typing_narrowing_typ_aux : forall Q E F X P e T,
-  typing (F ++ [(X, bind_typ Q)] ++ E) e T ->
-  sub E P Q ->
+(*
+Lemma typing_narrowing_typ_aux : forall Q Γ Δ X P e T,
+  (Δ ++ [(X, bind_typ Q)] ++ Γ) ⊢ e : T ->
+  Γ ⊢ P <: Q ->
   syn_cat_agree P Q ->
-  typing (F ++ [(X, bind_typ P)] ++ E) e T.
+  (Δ ++ [(X, bind_typ P)] ++ Γ) ⊢ e : T.
 Proof with simpl_env; eauto using
-    wf_env_narrowing_typ, wf_typ_narrowing_typ, sub_narrowing_typ,
+    wf_env_narrowing_typ, wf_typ_ignores_typ_bindings, sub_narrowing_typ,
     sub_weakening, type_from_wf_typ.
   intros *. intros HT HSub HAg.
   assert (type P) as Htype by eauto*.
@@ -205,7 +209,9 @@ Proof with simpl_env; eauto using
     + rewrite_parenthesise_binding.
       eapply H2...
 Qed.
+*)
 
+(*
 Lemma typing_narrowing_typ_tvars : forall (X Y : atom) E F x e T,
   typing (F ++ [(x, bind_typ X)] ++ E) e T ->
   sub E Y X ->
@@ -215,91 +221,158 @@ Proof with eauto.
   eapply typing_narrowing_typ_aux...
   constructor.
 Qed.
+*)
 
-Lemma typing_narrowing_typ : forall Q E F X C P e T,
-  typing (F ++ [(X, bind_typ Q)] ++ E) e T ->
-  sub E (typ_capt C P) Q ->
-  typing (F ++ [(X, bind_typ (typ_capt C P))] ++ E) e T.
-Proof with eauto.
-  intros* ? Hsub.
-  inversion Hsub; subst.
-  eapply typing_narrowing_typ_aux...
-  constructor.
+Lemma typing_narrowing_typ : forall D Q Γ Δ X C P e T,
+  (Δ ++ [(X, bind_typ (D # Q))] ++ Γ) ⊢ e : T ->
+  Γ ⊢ (C # P) <: (D # Q) ->
+  (Δ ++ [(X, bind_typ (C # P))] ++ Γ) ⊢ e : T.
+Proof with eauto*.
+  intros * Typ Sub.
+  assert (CsubD_PsubQ_WfC_WfD_PureP_PureQ : Γ ⊢ₛ C <: D /\ Γ ⊢ P <: Q /\ Γ ⊢ₛ C wf /\ Γ ⊢ₛ D wf /\ pure_type P /\ pure_type Q).
+  { dependent induction Sub...
+    destruct (IHSub D Q {} U)...
+    repeat split...
+    - assert (WfEU : Γ ⊢ ({} # U) wf) by (applys sub_regular Sub; assumption ).
+      inversion WfEU; subst.
+      rename select (Γ ⊢ U wf) into WfU.
+      apply sub_transitivity with (Q := U).
+      + eapply type_from_wf_typ...
+      + apply sub_tvar...
+      + applys IHSub...
+    - intros x xIn; exfalso; clear - xIn; fsetdec.
+  }
+  destruct CsubD_PsubQ_WfC_WfD_PureP_PureQ as [CsubD [PsubQ [WfC [WfD [PureP PureQ]]]]].
+  dependent induction Typ.
+  - Case "typing_var".
+    rename select (binds _ _ _) into Binds.
+    binds_cases Binds; simpl_env in *.
+    + eapply typing_var...
+      eapply wf_env_narrowing_typ...
+    + injection H1 as ReqQ C0eqD; subst.
+      apply typing_sub with (S := `cset_fvar` x # P).
+      * apply typing_var with (C := C)...
+        eapply wf_env_narrowing_typ...
+      * apply sub_capt...
+        -- apply subcapt_reflexivity...
+           econstructor; intros y yIn; assert (y = x) by fsetdec; subst; clear yIn...
+        -- rewrite_env (∅ ++ (Δ ++ [(x, bind_typ (C # P))]) ++ Γ).
+           apply sub_weakening...
+           simpl_env.
+           eapply wf_env_narrowing_typ...
+    + apply typing_var with (C := C0)...
+      eapply wf_env_narrowing_typ...
+  - Case "typing_abs".
+    pick fresh y and apply typing_abs...
+    + simpl_env in *.
+      eapply wf_typ_ignores_typ_bindings...
+    + rewrite_parenthesise_binding.
+      eapply H1...
+  - Case "typing_app".
+    eapply typing_app...
+  - Case "typing_let".
+    pick fresh y and apply typing_let...
+    rewrite_parenthesise_binding.
+    eapply H0...
+  - Case "typing_tabs".
+    pick fresh Y and apply typing_tabs...
+    + simpl_env in *.
+      eapply wf_typ_ignores_typ_bindings...
+    + rewrite_parenthesise_binding.
+      eapply H2...
+  - Case "typing_tapp".
+    eapply typing_tapp...
+    eapply sub_narrowing_typ...
+  - Case "typing_box".
+    apply typing_box...
+    simpl_env in *...
+  - Case "typing_unbox".
+    apply typing_unbox...
+    eapply wf_cset_narrowing_typ...
+    apply ok_from_wf_env.
+    eapply wf_env_narrowing_typ...
+    applys typing_regular Typ.
+  - Case "typing_sub".
+    apply typing_sub with (S := S)...
+    eapply sub_narrowing_typ...
 Qed.
-
 
 (* ********************************************************************** *)
 (** ** Inversion of typing (13) *)
 
-Lemma typing_inv_abs : forall E S1 e1 T,
-  typing E (exp_abs S1 e1) T ->
-  forall U1 U2 C, sub E T (typ_capt C (typ_arrow U1 U2)) ->
-     sub E U1 S1
-  /\ exists S2, exists L, forall x, x `notin` L ->
-    typing ([(x, bind_typ S1)] ++ E) (open_ve e1 x (`cset_fvar` x)) (open_ct S2 (`cset_fvar` x)) /\
-    wf_typ ([(x, bind_typ S1)] ++ E) (dom E `union` singleton x) (dom E) (open_ct U2 (`cset_fvar` x)) /\
-    sub ([(x, bind_typ U1)] ++ E) (open_ct S2 (`cset_fvar` x)) (open_ct U2 (`cset_fvar` x)).
+Lemma typing_inv_abs : forall Γ S1 e1 T,
+  Γ ⊢ (λ (S1) e1) : T ->
+  forall U1 U2 C, Γ ⊢ T <: (C # (∀ (U1) U2)) ->
+     Γ ⊢ U1 <: S1
+  /\ exists S2, exists L, forall x, x ∉ L ->
+    ([(x, bind_typ S1)] ++ Γ) ⊢ (open_ve e1 x (`cset_fvar` x)) : (open_ct S2 (`cset_fvar` x)) /\
+    ([(x, bind_typ S1)] ++ Γ) ⊢ (open_ct U2 (`cset_fvar` x)) wf /\
+    ([(x, bind_typ U1)] ++ Γ) ⊢ (open_ct S2 (`cset_fvar` x)) <: (open_ct U2 (`cset_fvar` x)).
 Proof with auto.
-  intros * Htyp.
-  dependent induction Htyp; intros U1 U2 C Hsub.
+  intros * Typ.
+  dependent induction Typ; intros U1 U2 D Sub.
   - Case "typing_abs".
-    inversion Hsub; subst.
-    inversion select (sub_pre _ _ _); subst.
+    inversion Sub; subst.
+    inversion select (_ ⊢ _ <: _); subst.
     split...
     exists T1.
-    exists (L `union` L0).
+    exists (L `u`A L0).
     intros y ?.
-    repeat split.
-    + apply H1...
-    + rewrite_nil_concat.
-      eapply wf_typ_ignores_typ_bindings.
-      apply H13...
-    + trivial...
-  - Case "typing_sub".
-    eauto using (sub_transitivity T).
-Qed.
-
-Lemma typing_inv_tabs : forall E S1 e1 T,
-  typing E (exp_tabs S1 e1) T ->
-  forall U1 U2 C, sub E T (typ_capt C (typ_all U1 U2)) ->
-     sub E U1 S1
-  /\ exists S2, exists L, forall X, X `notin` L ->
-     typing ([(X, bind_sub U1)] ++ E) (open_te e1 X) (open_tt S2 X)
-     /\ sub ([(X, bind_sub U1)] ++ E) (open_tt S2 X) (open_tt U2 X).
-Proof with simpl_env; auto.
-  intros * Htyp.
-  dependent induction Htyp; intros U1 U2 C Hsub.
-  - Case "typing_abs".
-    inversion Hsub; subst.
-    inversion select (sub_pre _ _ _); subst.
-    split...
-    exists T1.
-    exists (L `union` L0).
-    intros y ?.
+    rename select (forall x : atom, x ∉ L0 -> _) into Sub'.
+    specialize (Sub' y ltac:(fsetdec)).
     repeat split...
-    rewrite_env (empty ++ [(y, bind_sub U1)] ++ E).
-    eapply typing_narrowing with (Q := S1)...
+    + applys sub_regular Sub'.
+    + rewrite_nil_concat.
+      eapply sub_narrowing_typ with (CQ := C) (Q:= R)...
   - Case "typing_sub".
     eauto using (sub_transitivity T).
 Qed.
 
-Lemma typing_inv_let : forall E e k T,
-  typing E (exp_let e k) T ->
-  exists U,
-       typing E e U
-    /\ exists L, forall x, x `~in`A L ->
-         typing ([(x, bind_typ U)] ++ E) (open_ve k x (`cset_fvar` x)) T.
+Lemma typing_inv_tabs : forall Γ S1 e1 T,
+  Γ ⊢ (Λ [S1] e1) : T ->
+  forall U1 U2 C, Γ ⊢ T <: (C # (∀ [U1] U2)) ->
+     Γ ⊢ U1 <: S1
+  /\ exists S2, exists L, forall X, X ∉ L ->
+       ([(X, bind_sub U1)] ++ Γ) ⊢ (open_te e1 X) : (open_tt S2 X) /\
+       ([(X, bind_sub U1)] ++ Γ) ⊢ (open_tt S2 X) <: (open_tt U2 X).
+Proof with simpl_env; auto.
+  intros * Typ.
+  dependent induction Typ; intros U1 U2 D Sub.
+  - Case "typing_tabs".
+    inversion Sub; subst.
+    inversion select (_ ⊢ _ <: _); subst.
+    split...
+    exists T1.
+    exists (L `union` L0).
+    intros Y ?.
+    repeat split...
+    rewrite_nil_concat.
+    + eapply typing_narrowing with (Q := S1)...
+    + rename select (forall X : atom, X ∉ L0 -> _) into Sub'.
+      specialize (Sub' Y ltac:(fsetdec)).
+      rewrite_nil_concat.
+      apply sub_narrowing with (Q := S1)...
+  - Case "typing_sub".
+    eauto using (sub_transitivity T).
+Qed.
+
+Lemma typing_inv_let : forall Γ e k T,
+  Γ ⊢ (let= e in k) : T ->
+  exists C R,
+       Γ ⊢ e : (C # R)
+    /\ exists L, forall x, x ∉ L ->
+         ([(x, bind_typ (C # R))] ++ Γ) ⊢ (open_ve k x (`cset_fvar` x)) : T.
 Proof with eauto*.
   intros * Typ.
   dependent induction Typ...
-  destruct (IHTyp e k ltac:(reflexivity)) as [U [eTyp [L kTyp]]].
-  exists U.
+  destruct (IHTyp e k ltac:(reflexivity)) as [C [R [eTyp [L kTyp]]]].
+  exists C, R.
   split...
-  exists (L `u`A dom E).
+  exists (L `u`A dom Γ).
   intros y NotIn.
   specialize (kTyp y ltac:(clear - NotIn; fsetdec)).
   apply typing_sub with (S := S)...
-  rewrite_env (empty ++ [(y, bind_typ U)] ++ E).
+  rewrite_env (∅ ++ [(y, bind_typ (C # R))] ++ Γ).
   apply sub_weakening...
   apply wf_env_typ...
   applys typing_regular eTyp. 
